## $a_1=1$, $\displaystyle a_{n+1}=\frac{a_{n}}{1+\sqrt{a_{n}}}$, 证明 $\displaystyle\sum_{n=1}^{\infty} a_n<3$.

令 $b_n=1/a_n$ 得到 $b_1=1$, $b_{n+1}=b_n+\sqrt{b_n}$. 

设 $c_n=(pn+1-p)^2$, 并令 $c_{n+1}\le c_n+\sqrt{c_n}$, 这将使得 $b_n\ge c_n$, 从而 $\displaystyle\sum_{n=1}^{\infty} a_n\le \sum_{n=1}^\infty \frac{1}{c_n}$.

将 $c_n=(pn+1-p)^2$ 代入 $c_{n+1}\le c_n+\sqrt{c_n}$ 得到 $(p-2p^2)n+p^2-3p+1\ge 0$. 为了让它对任意的 $n$ 成立, 可以令 $\displaystyle p<\frac{1}{2}$ 且不等式在 $n=1$ 时成立. 将 $n=1$ 代入得 $p^2+2p\le 1$, 取 $p$ 使得等号成立并验证 $\displaystyle p<\frac{1}{2}$. 此时 $\displaystyle\sum_{n=1}^\infty \frac{1}{c_n} = 1 + \frac{1}{p^2} \sum_{n=1}^\infty \frac{1}{(n+\frac{1}{p})^2} < 1 + \frac{1}{p^2}\frac{1}{\frac{1}{2}+\frac{1}{p}} = 1 + \frac{2}{p^2+2p} = 3$.

上述求和利用了 $\displaystyle\frac{1}{x^2} < \frac{1}{x-\frac{1}{2}} - \frac{1}{x+\frac{1}{2}}$.
